snap

experiments/HandleAwayEff.fst
@@ -7,6 +7,15 @@ open FStar.Tactics.Typeclasses
 
 assume type beta : Type u#0
 
+let pure_wp (a: Type) = wp:pure_wp' a{pure_wp_monotonic0 a wp}
+
+let pure_return (x:'a) : pure_wp 'a =
+  pure_return 'a x
+
+let pure_bind (m:pure_wp 'a) (k:'a -> pure_wp 'b) : pure_wp 'b =
+  FStar.Monotonic.Pure.elim_pure_wp_monotonicity_forall ();
+  pure_bind_wp _ _ (as_pure_wp m) (fun x -> as_pure_wp (k x))
+  
 (** *** Source monad : a Dijkstra Monad **)
 noeq
 type free_req (a:Type u#a) : Type u#(a+1) = 
@@ -16,20 +25,20 @@ type free_req (a:Type u#a) : Type u#(a+1) =
 
 let rec theta (m:free_req 'a) : pure_wp 'a =
   match m with
-  | Return x -> pure_return _ x
+  | Return x -> pure_return x
   | Op k ->
-    pure_bind_wp _ _ (as_pure_wp (fun p -> forall x. p x)) (fun x -> theta (k x))
-  | Require pre k -> pure_bind_wp _ _ (as_pure_wp (fun p -> pre /\ p (() <: squash pre))) (fun r -> theta (k r))
+    pure_bind (fun p -> forall x. p x) (fun x -> theta (k x))
+  | Require pre k -> pure_bind (fun p -> pre /\ p (() <: squash pre)) (fun r -> theta (k r))
 
 let dm (a:Type) (wp:pure_wp a) =
   m:(free_req a){forall p. wp p ==> theta m p}
 
-let dm_return (x:'a) : dm 'a (pure_return 'a x) = Return x
+let dm_return (x:'a) : dm 'a (pure_return x) = Return x
 
 let dm_bind (#a:Type u#a) (#b:Type u#b) (#wp1:pure_wp a) (#wp2:a -> pure_wp b)
   (m:dm a wp1)
   (k:(x:a -> dm b (wp2 x))) :
-  dm b (pure_bind_wp a b wp1 wp2) =
+  dm b (pure_bind wp1 wp2) =
   admit ()
 
 let dm_subcomp (#a:Type u#a) (#wp1:pure_wp a) (#wp2:pure_wp a) (m:dm a wp1) : Pure (dm a wp2) (requires (forall p. wp2 p ==> wp1 p)) (ensures fun _ -> True) = m
@@ -40,12 +49,26 @@ instance source_int : source int = { _empty = () }
 
 instance source_pair (t1:Type) {| source t1 |} (t2:Type) {| source t2 |} : source (t1 * t2) = { _empty = () }
 
-instance source_arrow (t1:Type) {| source t1 |} (t2:Type) {| source t2 |} (wp:t1 -> pure_wp t2) : source (x:t1 -> dm t2 (wp x)) = { _empty = () }
+instance source_arrow
+  (t1:Type) {| source t1 |}
+  (t2:t1 -> Type) {| (x:t1) -> source (t2 x) |}
+  (wp:(x:t1) -> pure_wp (t2 x)) : 
+  source (x:t1 -> dm (t2 x) (wp x)) = { _empty = () }
 
-let test0 l: source (x:int -> dm int (as_pure_wp (fun p -> x > 5 /\ (forall r. p r)))) =
-  source_arrow int int (fun x -> (as_pure_wp (fun p -> x > 5 /\ (forall r. p r))))
+let test0 : source (x:int -> dm int (as_pure_wp (fun p -> x > 5 /\ (forall r. p r)))) =
+  source_arrow int (fun _ -> int) (fun x -> (as_pure_wp (fun p -> x > 5 /\ (forall r. p r))))
 
-//let test : source (x:int -> dm (y:int -> dm int (as_pure_wp (fun p -> x == y /\ (forall r. p r)))) (as_pure_wp (fun p -> x > 5 /\ (forall r. p r)))) = solve
+let test1 : source (x:int -> dm (y:int -> dm int (fun p -> x == y /\ (forall r. p r))) (fun p -> x > 5 /\ (forall r. p r))) =
+  source_arrow
+    int _ #(fun x -> source_arrow int (fun _ -> int)
+    (fun y -> as_pure_wp (fun p -> x == y /\ (forall r. p r))))
+    (fun x -> as_pure_wp (fun p -> x > 5 /\ (forall r. p r)))
+
+let test2 : source ((y:int -> dm int (fun p -> y > 2 /\ (forall r. p r))) -> dm int (fun p -> (forall r. p r))) =
+  source_arrow
+    _ #(source_arrow int (fun _ -> int) (fun y p -> y > 2 /\ (forall r. p r)))
+    (fun _ -> int)
+    (fun _ p -> (forall r. p r))
 
 (** *** Target monad : a Free Monad with less constructors **)
 noeq
@@ -72,21 +95,21 @@ instance target_arrow (t1:Type) {| target t1 |} (t2:Type) {| target t2 |} : targ
 let behS (m:dm 'a 'wp) = theta m
 let rec behT (m:free 'a) : pure_wp 'a = 
   match m with
-  | Ret x -> pure_return _ x
+  | Ret x -> pure_return x
   | Call k ->
-    pure_bind_wp _ _ (as_pure_wp (fun p -> forall x. p x)) (fun x -> behT (k x))
+    pure_bind (fun p -> forall x. p x) (fun x -> behT (k x))
 
 let eq_beh (rel:'a -> 'b -> Type0) (w1:pure_wp 'a) (w2:pure_wp 'b): Type0 =
   forall p1 p2. (forall r1 r2. r1 `rel` r2 ==> (p1 r1 <==> p2 r2)) ==> (w1 p1 <==> w2 p2)
 // TODO: figure out how to define this equivalence
 
 
-let rec lift_m (m:free 'a) : dm 'a (as_pure_wp (fun p -> forall r. p r)) =
+let rec lift_m (m:free 'a) : dm 'a (fun p -> forall r. p r) =
   match m with
   | Ret x -> Return x
   | Call k -> Op (fun x -> lift_m (k x))
 
-let rec handle_m (m:dm 'a (as_pure_wp (fun p -> forall r. p r))) : free 'a =
+let rec handle_m (m:dm 'a (fun p -> forall r. p r)) : free 'a =
   match m with
   | Return x -> Ret x
   | Require pre k -> begin
@@ -107,7 +130,7 @@ class liftable (t:Type u#a) = {
 
   lift : t -> s;
 
-//  lem1 : w:free t -> rel:(t -> s -> Type0) -> Lemma ((behT w) `eq_beh rel` (behS (dm_bind (lift_m w) (fun r -> dm_return (lift r)))))
+  lem1 : w:free t -> rel:(t -> s -> Type0) -> Lemma ((behT w) `eq_beh rel` (behS (dm_bind (lift_m w) (fun r -> dm_return (lift r)))))
 }
 
 class handleable (t:Type u#a) = {
@@ -128,6 +151,7 @@ instance liftable_int : liftable int = {
   s_tc = solve;
 
   lift = (fun x -> x);
+  lem1 = (fun x rel -> admit ())
 }
 
 instance liftable_pair (t1 t2:Type) {| c1:liftable t1 |} {| c2:liftable t2 |} : liftable (t1 * t2) = {
@@ -136,16 +160,18 @@ instance liftable_pair (t1 t2:Type) {| c1:liftable t1 |} {| c2:liftable t2 |} : 
   s_tc = source_pair c1.s #c1.s_tc c2.s #c2.s_tc;
 
   lift = (fun (x, y) -> (lift x, lift y));
+  lem1 = (fun x rel -> admit ())
 }
 
 instance liftable_arrow (t1 t2:Type) {| c1:handleable t1 |} {| c2:liftable t2 |} : liftable (t1 -> free t2) = {
   t_tc = target_arrow t1 #c1.t_tc t2 #c2.t_tc;
-  s = c1.s -> dm c2.s (as_pure_wp (fun p -> forall r. p r));
-  s_tc = source_arrow c1.s #c1.s_tc c2.s #c2.s_tc (fun x -> as_pure_wp (fun p -> forall r. p r));
+  s = c1.s -> dm c2.s (fun p -> forall r. p r);
+  s_tc = source_arrow c1.s #c1.s_tc (fun _ -> c2.s) #(fun _ -> c2.s_tc) (fun x p -> forall r. p r);
 
   lift = (fun (f:t1 -> free t2) (x:c1.s) -> 
     dm_bind (lift_m #t2 (f (handle x))) (fun (r:t2) -> dm_return (c2.lift r))
   );
+  lem1 = (fun x rel -> admit ())
 }
 
 instance handleable_int : handleable int = {
@@ -158,15 +184,15 @@ instance handleable_int : handleable int = {
 
 instance handleable_arrow (t1 t2:Type) {| c1:liftable t1 |} {| c2:handleable t2 |} : handleable (t1 -> free t2) = {
   t_tc = target_arrow t1 #c1.t_tc t2 #c2.t_tc;
-  s = c1.s -> dm c2.s (as_pure_wp (fun p -> forall r. p r));
-  s_tc = source_arrow c1.s #c1.s_tc c2.s #c2.s_tc (fun x -> as_pure_wp (fun p -> forall r. p r));
+  s = c1.s -> dm c2.s (fun p -> forall r. p r);
+  s_tc = source_arrow c1.s #c1.s_tc (fun _ -> c2.s) #(fun _ -> c2.s_tc) (fun x p -> forall r. p r);
 
   handle = (fun f (x:t1) ->
     free_bind (handle_m (f (lift x))) (fun r -> free_return (c2.handle r))
   )
 }
 
-let sc (ps:(int -> dm int (as_pure_wp (fun p -> forall r. p r))) -> dm int (as_pure_wp (fun p -> forall r. p r))) (ct:int -> free int) : Type0 =
+let sc (ps:(int -> dm int (fun p -> forall r. p r)) -> dm int (fun p -> forall r. p r)) (ct:int -> free int) : Type0 =
   behS (ps (lift ct)) `eq_beh (==)` behT ((fun cb -> free_bind (handle_m (ps (lift cb))) (fun r -> free_return (handle r))) ct)
 
 open FStar.Tactics
@@ -179,23 +205,23 @@ let sc_proof ps ct : Lemma (sc ps ct)
     mapply x;
     norm [delta_only [`%sc]];
     explode ();
+    dump "H";
     tadmit ();
     tadmit ()
   )
   = ()
 
-let sc' (ct:(int -> free int) -> free int) (ps:int -> dm int (as_pure_wp (fun p -> forall r. p r))) : Type0 =
-  behS (dm_bind (lift_m (ct ((handleable_arrow int int).handle ps))) (fun r -> dm_return (lift r))) `eq_beh (==)` behT (ct (handle ps))
+let sc' (ct:(int -> free int) -> free int) (ps:int -> dm int (fun p -> forall r. p r)) : Type0 =
+  behT (ct (handle ps)) `eq_beh (==)`
+  behS (dm_bind (lift_m (ct ((handleable_arrow int int).handle ps))) (fun r -> dm_return (lift r))) 
 
 let sc_proof' ps ct : Lemma (sc' ct ps)
   by (
     explode ();
-    let x = nth_binder (-2) in
+    let x = nth_binder (-3) in
     let x = instantiate x (fresh_uvar None) in
     mapply x;
     norm [delta_only [`%sc']];
-    explode ();
-    tadmit ();
-    tadmit ()
+    assumption ()
   )
-  = ()
+  = lem1 (ct (handle ps)) (==)
